{
 "cells": [
  {
   "cell_type": "markdown",
   "id": "185db601",
   "metadata": {},
   "source": [
    "# 1.\n",
    "\n",
    "Recall the definition of a rational number, denoted as $\\mathbb{Q}$. Prove that the Euler's number $e=\\sum ^{\\infty} _{k=0}\\frac{1}{k!}\\notin \\mathbb{Q}$. A factorial is defined as $k!=(k)(k-1)(k-2)(k-3)...,\\forall k\\in \\mathbb{Z}^+$, note that $0!=1$. Furthermore, a sum notation $\\sum ^\\infty _{k=0} k=0+1+2+3+...+...$"
   ]
  },
  {
   "cell_type": "markdown",
   "id": "87c81a4b",
   "metadata": {},
   "source": [
    "### Proof:\n",
    "\n",
    "Assume that $e$ is rational.\n",
    "\n",
    "There exist coprime integers $m$ and $n$ (let $n\\in \\mathbb{Z}^+$) such that:\n",
    "$$\n",
    "\\frac{m}{n} = e = \\sum ^\\infty _{i=0} \\frac{1}{i!}\n",
    "$$\n",
    "\n",
    "Multiplying both sides by $n!$, note that:\n",
    "$$\n",
    "\\frac{m}{n}n!=n!\\sum ^\\infty _{i=0} \\frac{1}{i!}=\\left(\\frac{n!}{0!}+\\frac{n!}{1!}+\\frac{n!}{2!}+\\cdots+\\frac{n!}{n!}\\right)+\\left(\\frac{n!}{(n+1)!}+\\frac{n!}{(n+2)!}+\\cdots\\right)\n",
    "$$\n",
    "\n",
    "Hence:\n",
    "$$\n",
    "m(n-1)!-\\left(\\frac{n!}{0!}+\\frac{n!}{1!}+\\frac{n!}{2!}+\\cdots+\\frac{n!}{n!}\\right)=\\frac{1}{(n+1)}+\\frac{1}{(n+1)(n+2)}+\\frac{1}{(n+1)(n+2)(n+3)}+\\cdots\n",
    "$$\n",
    "$$\n",
    "\\hspace{6cm}<\\frac{1}{(n+1)}+\\frac{1}{(n+1)(n+1)}+\\frac{1}{(n+1)(n+1)(n+1)}+\\cdots\n",
    "$$\n",
    "$$\n",
    "=\\sum ^\\infty _{i=0}\\left(\\frac{1}{n+1}\\right)^{(i+1)}\n",
    "$$\n",
    "$$\n",
    "=\\frac{\\frac{1}{n+1}}{1-\\frac{1}{n+1}}=\\frac{1}{n}\\leq 1\n",
    "$$\n",
    "\n",
    "Note that the quantity on the left hand side is strictly positive, since it is equal to:\n",
    "$$\n",
    "\\frac{1}{(n+1)}+\\frac{1}{(n+1)(n+2)}+\\frac{1}{(n+1)(n+2)(n+3)}+\\cdots\n",
    "$$\n",
    "...which is strictly positive.\n",
    "\n",
    "Thus,\n",
    "$$\n",
    "m(n-1)!-\\left(\\frac{n!}{0!}+\\frac{n!}{1!}+\\frac{n!}{2!}+\\cdots+\\frac{n!}{n!}\\right)\n",
    "$$\n",
    "must be a strictly positive integer that is less than 1.\n",
    "\n",
    "Because this is a contradiction, $e$ must be irrational."
   ]
  },
  {
   "cell_type": "markdown",
   "id": "b26dd070",
   "metadata": {},
   "source": [
    "# 2.\n",
    "\n",
    "Prove Minkowski's Inequality for sums $\\forall p>1, (a_k, b_k)>0:$\n",
    "$$\\begin{bmatrix}\\sum ^n _{k=1}|a_k+b_k|^p\\end{bmatrix}^\\frac{1}{p}\\leq \\begin{bmatrix}\\sum^n _{k=1}|a_k|^p\\end{bmatrix}^\\frac{1}{p}+\\begin{bmatrix}\\sum^n _{k=1}|b_k|^p\\end{bmatrix}^\\frac{1}{p}$$"
   ]
  },
  {
   "cell_type": "markdown",
   "id": "a6d40137",
   "metadata": {},
   "source": [
    "### Proof\n",
    "\n",
    "#### Step 1: Laws of Exponents (Power raised to a power):\n",
    "\n",
    "- Let $n = $ any base number, then ${(n^p)}^\\frac{1}{p}=n$\n",
    "- We know that ${(n^p)}^\\frac{1}{p}=n$ for any base number $n$, which implies that the $p$-th root of $n^p$ is $n$. Applying this to the sums of $|a_k|^p$ and $|b_k|^p$, we have:\n",
    "\n",
    "\\begin{gather} \n",
    "\\Sigma_{k=1}^n |a_k + b_k|\n",
    "\\leq\n",
    "\\Sigma_{k=1}^n |a_k|\n",
    "+\n",
    "\\Sigma_{k=1}^n |b_k|\n",
    "\\end{gather}\n",
    "\n",
    "#### Step 2: Property of Summation (Addition)\n",
    "\n",
    "\\begin{gather} \n",
    "\\Sigma_{k=1}^n |a_k + b_k|\n",
    "\\leq\n",
    "\\Sigma_{k=1}^n |a_k| + |b_k|\n",
    "\\end{gather}\n",
    "\n",
    "#### Step 3: Prove by Triangle Inequality\n",
    "\n",
    "- Disregarding the Sigma Notation we get:\n",
    "\\begin{gather}\n",
    "|a_k + b_k|\n",
    "\\leq\n",
    "|a_k| + b_k| \n",
    "\\end{gather}\n",
    "\n",
    "- Since, $(a_k, b_k) > 0$, then $(a + b) = a + b$, and $|a| = a_k$, $|b| = b$:\n",
    "- Substitute:\n",
    "\\begin{gather}\n",
    "|a + b| = a + b = |a| + |b|\n",
    "\\end{gather}\n",
    "\n",
    "\n",
    "Thus,\n",
    "\n",
    "$$\\begin{bmatrix}\\sum ^n _{k=1}|a_k+b_k|^p\\end{bmatrix}^\\frac{1}{p}\\leq \\begin{bmatrix}\\sum^n _{k=1}|a_k|^p\\end{bmatrix}^\\frac{1}{p}+\\begin{bmatrix}\\sum^n _{k=1}|b_k|^p\\end{bmatrix}^\\frac{1}{p}$$"
   ]
  },
  {
   "cell_type": "markdown",
   "id": "6736225c",
   "metadata": {},
   "source": [
    "# 3.\n",
    "\n",
    "Prove the triangle inequality $|x+y|\\leq |x|+|y|, \\forall(x,y)\\in\\mathbb{R}$"
   ]
  },
  {
   "cell_type": "markdown",
   "id": "51617ca7",
   "metadata": {},
   "source": [
    "### Proof:\n",
    "We must first prove that $\\left(|x|+|y|\\right)^2\\geq|x+y|^2$. Note that $\\forall n\\in\\mathbb{R}$, $|n|^2 = n^2$.\n",
    "\n",
    "$$\n",
    "\\left(|x| + |y|\\right)^2 = |x|^2 + 2|x||y| + |y|^2\n",
    "$$\n",
    "\n",
    "Because $|x|\\geq x$ and $|y|\\geq y$:\n",
    "\n",
    "$$\n",
    "|x|^2 + 2|x||y| + |y|^2\\geq x^2 + 2xy + y^2 = \\left(a + b\\right)^2 = |a+b|^2\n",
    "$$\n",
    "\n",
    "So,\n",
    "$$\n",
    "(|a|+|b|)^2\\geq |a+b|^2\n",
    "$$\n",
    "\n",
    "Therefore, getting the square root of the inequality above,\n",
    "$$\n",
    "|a|+|b|\\geq|a+b|\n",
    "$$\n",
    "\n",
    "That is,\n",
    "$$\n",
    "|a+b|\\leq|a|+|b|\n",
    "$$"
   ]
  },
  {
   "cell_type": "markdown",
   "id": "52dba81a",
   "metadata": {},
   "source": [
    "# 4.\n",
    "\n",
    "Prove Sedrakayan's Lemma $\\forall u_i, v_i\\in\\mathbb{R}^+$:\n",
    "$$\\frac{(\\sum ^n _{i=1}u_i)^2}{\\sum ^n _{i=1}v_i}\\leq\\sum ^n _{i=1}\\frac{(u_i)^2}{v_i}$$"
   ]
  },
  {
   "cell_type": "markdown",
   "id": "5d75b058",
   "metadata": {},
   "source": [
    "### Proof:\n",
    "\n",
    "#### Step 1:\n",
    "\n",
    "To prove Sedrakayanâ€™s Lemma directly, we need to demonstrate that for all $(u_i, v_i \\in \\mathbb{R}^+)$, the inequality\n",
    "\n",
    "$$\\left(\\frac{\\sum_{i=1}^n u_i}{\\sum_{i=1}^n v_i}\\right)^2 \\leq \\frac{\\sum_{i=1}^n (u_i)^2}{v_i}$$\n",
    "\n",
    "holds true. \n",
    "\n",
    "#### Step 2:\n",
    "\n",
    "The ***Cauchy-Schwarz Inequality*** states that for any real numbers $(a_i)$ and $(b_i)$, \n",
    "\n",
    "$$\\left(\\sum_{i=1}^n a_i b_i\\right)^2 \\leq \\left(\\sum_{i=1}^n (a_i)^2\\right) \\left(\\sum_{i=1}^n (b_i)^2\\right)$$\n",
    "\n",
    "#### Step 3:\n",
    "\n",
    "Let $a_i = \\sqrt{u_i}$ and $b_i = \\frac{1}{\\sqrt{v_i}}$. Then, the Cauchy-Schwarz Inequality becomes\n",
    "\n",
    "$$\\left(\\sum_{i=1}^n \\sqrt{u_i} \\cdot \\frac{1}{\\sqrt{v_i}}\\right)^2 \\leq \\left(\\sum_{i=1}^n u_i\\right) \\left(\\sum_{i=1}^n \\frac{1}{v_i}\\right)$$\n",
    "\n",
    "#### Step 4:\n",
    "\n",
    "The *left-hand side* simplifies to \n",
    "\n",
    "$$\\left(\\frac{\\sum_{i=1}^n u_i}{\\sum_{i=1}^n v_i}\\right)^2$$\n",
    "\n",
    "#### Step 5:\n",
    "\n",
    "The *right-hand side* simplifies to \n",
    "\n",
    "$$\\frac{\\sum_{i=1}^n (u_i)^2}{v_i}$$\n",
    "\n",
    "So,\n",
    "\n",
    "$$\\left(\\frac{\\sum_{i=1}^n u_i}{\\sum_{i=1}^n v_i}\\right)^2 \\leq \\frac{\\sum_{i=1}^n (u_i)^2}{v_i}$$\n",
    "\n",
    "That is,\n",
    "\n",
    "$$\\frac{(\\sum ^n _{i=1}u_i)^2}{\\sum ^n _{i=1}v_i}\\leq\\sum ^n _{i=1}\\frac{(u_i)^2}{v_i}$$"
   ]
  },
  {
   "cell_type": "markdown",
   "id": "c36fda5d",
   "metadata": {},
   "source": [
    "# Extra problems:"
   ]
  },
  {
   "cell_type": "markdown",
   "id": "ce28ffd5",
   "metadata": {},
   "source": [
    "1. Consider the functions $f(x) = 2x+1$, $g(x)=2y-1$, $j(x) = |f(x)+g(x)|$, and $h(x) = j(x)^2$, show for the following inequality that:\n",
    "\n",
    "\\begin{gather}\n",
    "\\sqrt{|f(x)|^2} \\geq \\sqrt{h(x)} - \\sqrt{|g(x)|^2}, \\forall (x,y) \\in \\mathbb{Z}^+\n",
    "\\end{gather}"
   ]
  },
  {
   "cell_type": "markdown",
   "id": "05199c33",
   "metadata": {},
   "source": [
    "With the given functions, we can substitute $f(x)$ and $g(x)$ into $j(x)$:\n",
    "$$\n",
    "    j(x) = |(2x + 1) + (2y - 1)| = |2x + 2y| = 2|x + y|.\n",
    "$$\n",
    "\n",
    "With this, we can also find $h(x)$:\n",
    "$$\n",
    "    h(x) = j(x)^2 = (2|x + y|)^2 = 4(x + y)^2.\n",
    "$$\n",
    "\n",
    "We can then simplify the inequality by substituting the function names:\n",
    "$$\n",
    "    \\sqrt{h(x)} = \\sqrt{4(x + y)^2} = 2|x + y|.\n",
    "$$\n",
    "\n",
    "$$\n",
    "    \\sqrt{|f(x)|^2} = \\sqrt{(2x + 1)^2} = |2x + 1|\n",
    "$$\n",
    "\n",
    "$$\n",
    "    \\sqrt{|g(x)|^2} = \\sqrt{(2y - 1)^2} = |2y - 1|\n",
    "$$\n",
    "\n",
    "So we have:\n",
    "\n",
    "$$\n",
    "    |2x + 1| \\geq 2|x + y| - |2y - 1|\n",
    "$$\n",
    "\n",
    "When analyzing the different absolute values in the equation as well as from the given, we can see that:\n",
    "- For $( 2x + 1 )$, it's always positive for $( x \\in \\mathbb{Z}^+ )$, hence $( |2x + 1| = 2x + 1 )$.\n",
    "- For $( 2y - 1 )$, if $( y \\geq 1 )$, then $( |2y - 1| = 2y - 1)$\n",
    "- For $(x + y)$, since $(x,y) \\in \\mathbb{Z}^+$, then $|x + y| = (x + y)$\n",
    "\n",
    "Therefore, the equality can be simplified down to:\n",
    "$$\n",
    "    2x + 1 \\geq 2(x + y) - (2y - 1)\n",
    "$$\n",
    "\n",
    "$$\n",
    "    2x + 1 \\geq 2x + 2y - 2y + 1\n",
    "$$\n",
    "\n",
    "$$\n",
    "    2x + 1 \\geq 2x + 1\n",
    "$$\n",
    "\n",
    "Therefore, the original inequality is proven since $2x + 1 \\geq 2x + 1$ is always true regardless of the value of x."
   ]
  },
  {
   "cell_type": "markdown",
   "id": "72bd3bc5",
   "metadata": {},
   "source": [
    "2. Prove Sedrakayan's Lemma if $u_i, v_i$ are square roots of an even integers:\n",
    "\\begin{gather}\n",
    "\\frac{(\\Sigma_{i=1}^n u_i)^2}{\\Sigma_{i=1}^n v_i}\n",
    "\\leq\n",
    "\\Sigma_{i=1}^n \\frac{(u_i)^2}{v_i}\n",
    "\\end{gather}"
   ]
  },
  {
   "cell_type": "markdown",
   "id": "f64f715b",
   "metadata": {},
   "source": [
    "To prove Sedrakayan's Lemma when $ u_i $ and $ v_i $ are square roots of even integers:\n",
    "\n",
    "Let $ u_i = \\sqrt{2a_i} $ and $ v_i = \\sqrt{2b_i} $, where $ a_i $ and $ b_i $ are positive integers. We need to show:\n",
    "\n",
    "$$\n",
    "\\frac{\\left( \\sum_{i=1}^n \\sqrt{2a_i} \\right)^2}{\\sum_{i=1}^n \\sqrt{2b_i}} \\leq \\sum_{i=1}^n \\frac{(2a_i)}{(2b_i)}\n",
    "$$\n",
    "\n",
    "#### Step 1: Expand the terms\n",
    "\n",
    "Expanding the terms, we get:\n",
    "\n",
    "$$\n",
    "\\frac{\\left( \\sum_{i=1}^n \\sqrt{2a_i} \\right)^2}{\\sum_{i=1}^n \\sqrt{2b_i}} = \\frac{\\left( \\sum_{i=1}^n \\sqrt{2a_i} \\right) \\left( \\sum_{i=1}^n \\sqrt{2a_i} \\right)}{\\sum_{i=1}^n \\sqrt{2b_i}}\n",
    ", \\quad\n",
    "\\sum_{i=1}^n \\frac{(2a_i)}{(2b_i)} = \\sum_{i=1}^n \\frac{2a_i}{2b_i}\n",
    "$$\n",
    "\n",
    "\n",
    "#### Step 2: Rewrite\n",
    "\n",
    "Since $ \\sqrt{2a_i} $ and $ \\sqrt{2b_i} $ are positive, we can rewrite the inequality as:\n",
    "\n",
    "$$\n",
    "\\frac{\\left( \\sum_{i=1}^n \\sqrt{2a_i} \\right)^2}{\\sum_{i=1}^n \\sqrt{2b_i}} \\leq \\sum_{i=1}^n \\frac{\\sqrt{2a_i}^2}{\\sqrt{2b_i}}\n",
    "$$\n",
    "\n",
    "#### Step 3: Consider the identity:\n",
    "\n",
    "Now, consider the following identity:\n",
    "\n",
    "$$\n",
    "\\left( \\sum_{i=1}^n x_i \\right)^2 = \\sum_{i=1}^n x_i^2 + 2 \\sum_{1 \\leq i < j \\leq n} x_i x_j\n",
    "$$\n",
    "\n",
    "#### Step 4: Apply the identity\n",
    "\n",
    "Applying this identity to the numerator, we get:\n",
    "\n",
    "$$\n",
    "\\frac{\\left( \\sum_{i=1}^n \\sqrt{2a_i} \\right)^2}{\\sum_{i=1}^n \\sqrt{2b_i}} = \\frac{\\sum_{i=1}^n (2a_i) + 2 \\sum_{1 \\leq i < j \\leq n} \\sqrt{2a_i} \\sqrt{2a_j}}{\\sum_{i=1}^n \\sqrt{2b_i}}\n",
    "$$\n",
    "\n",
    "#### Step 5: Consider the following:\n",
    "\n",
    "Since $2a_i$ and $2b_i$ are even integers, $2 \\sum_{1 \\leq i < j \\leq n} \\sqrt{2a_i} \\sqrt{2a_j}$ is also even.\n",
    "\n",
    "Now, we have:\n",
    "\n",
    "$$\n",
    "\\frac{\\sum_{i=1}^n (2a_i)}{\\sum_{i=1}^n \\sqrt{2b_i}} + \\frac{2 \\sum_{1 \\leq i < j \\leq n} \\sqrt{2a_i} \\sqrt{2a_j}}{\\sum_{i=1}^n \\sqrt{2b_i}} \\leq \\sum_{i=1}^n \\frac{(2a_i)}{\\sqrt{2b_i}}\n",
    "$$\n",
    "\n",
    "#### Step 6: Simplify the expression\n",
    "$$\n",
    "\\frac{\\sum_{i=1}^n (2a_i)}{\\sum_{i=1}^n \\sqrt{2b_i}} \\leq \\sum_{i=1}^n \\frac{(2a_i)}{\\sqrt{2b_i}}\n",
    "$$\n",
    "\n",
    "Since both sides of the inequality are non-negative, and the numerator of the left-hand side contains the terms of the denominator of the right-hand side, the inequality holds true. Therefore, Sedrakayan's Lemma is proven for $ u_i $ and $ v_i $ being square roots of even integers."
   ]
  }
 ],
 "metadata": {
  "kernelspec": {
   "display_name": "Python 3 (ipykernel)",
   "language": "python",
   "name": "python3"
  },
  "language_info": {
   "codemirror_mode": {
    "name": "ipython",
    "version": 3
   },
   "file_extension": ".py",
   "mimetype": "text/x-python",
   "name": "python",
   "nbconvert_exporter": "python",
   "pygments_lexer": "ipython3",
   "version": "3.11.5"
  }
 },
 "nbformat": 4,
 "nbformat_minor": 5
}
